Locally Nameless: Nice notation and tactic for freshness. Remove dead code and refactor proofs. Experiment with bidirectional typing and evaluation contexts.

LocallyNameless/Atom.v
@@ -1,35 +1,94 @@
-Require Import
+Require Export
   List
   Coq.Classes.DecidableClass
   Lia.
 
 Import ListNotations.
 
+Arguments decide : simpl never.
+
+Ltac decide_all :=
+repeat match goal with
+| |- context [decide (?x = ?x)] => rewrite Decidable_complete by easy
+| |- context [decide (?x = ?y)] => decide (x = y); subst; cbn; try easy
+end.
+
+(** * Class of Atom-like types *)
+
 Class isAtom (Atom : Type) : Type :=
 {
   Decidable_isAtom :: forall x y : Atom, Decidable (x = y);
   fresh : list Atom -> Atom;
   fresh_spec : forall l : list Atom, ~ In (fresh l) l;
+  Fresh (x : Atom) (l : list Atom) : Prop := ~ In x l;
 }.
 
-Inductive Atom : Type :=
-| Fresh : list Atom -> Atom.
+Notation "x # l" := (Fresh x l) (at level 68).
 
-Definition out (x : Atom) : list Atom :=
-match x with
-| Fresh l => l
+(** * Freshness tactics *)
+
+Lemma incl_app_l :
+  forall {A : Type} (l1 l2 l3 : list A),
+    incl l1 l2 -> incl l1 (l2 ++ l3).
+Proof.
+  unfold incl.
+  intros.
+  rewrite in_app_iff.
+  now firstorder.
+Qed.
+
+Lemma incl_app_r :
+  forall {A : Type} (l1 l2 l3 : list A),
+    incl l1 l3 -> incl l1 (l2 ++ l3).
+Proof.
+  unfold incl.
+  intros.
+  rewrite in_app_iff.
+  now firstorder.
+Qed.
+
+Section sec_Fresh_lemmas.
+
+Context
+  {Atom : Type}
+  {isAtom_Atom : isAtom Atom}.
+
+Lemma Fresh_incl :
+  forall (x : Atom) (l1 l2 : list Atom),
+    incl l1 l2 -> x # l2 -> x # l1.
+Proof.
+  now firstorder.
+Qed.
+
+Lemma fresh_incl :
+  forall (l1 l2 : list Atom),
+    incl l1 l2 -> fresh l2 # l1.
+Proof.
+  intros.
+  eapply Fresh_incl with l2; [easy |].
+  now apply fresh_spec.
+Qed.
+
+End sec_Fresh_lemmas.
+
+Ltac solve_fresh :=
+repeat match goal with
+| |- fresh _ # _ => apply fresh_incl
+(* | |- Fresh (fresh _) _ => apply fresh_incl *)
+(* | |- ~ In (fresh _) _ => apply fresh_incl *)
+| |- incl ?l ?l => apply incl_refl
+| |- incl _ _ => now apply incl_app_l
+| |- incl _ _ => apply incl_app_r
 end.
 
-(*
-Inductive Atom : Type := Fresh
-{
-  out : list Atom;
-}.
-*)
+(** * Inductive Atoms *)
+
+Inductive Atom : Type :=
+| mkAtom : list Atom -> Atom.
 
 Fixpoint size (x : Atom) : nat :=
 match x with
-| Fresh l => 1 + fold_right (fun h t => size h + t) 0 l
+| mkAtom l => 1 + fold_right (fun h t => size h + t) 0 l
 end.
 
 Definition sizes l := 1 + fold_right (fun h t => size h + t) 0 l.
@@ -39,7 +98,7 @@ Proof.
   refine
   (
     match x, y with
-    | Fresh lx, Fresh ly =>
+    | mkAtom lx, mkAtom ly =>
       match list_eq_dec eq_dec_Atom lx ly with
       | left eq => _
       | right neq => _
@@ -76,13 +135,15 @@ Qed.
 
 #[export, refine] Instance isAtom_Atom : isAtom Atom :=
 {
-  fresh := Fresh;
+  fresh := mkAtom;
 }.
 Proof.
   intros l Hin.
   apply In_size in Hin. cbn in Hin.
   now lia.
 Defined.
+
+(** * Natural numbers as atoms *)
 
 Fixpoint fresh_nat (l : list nat) : nat :=
 match l with
